dataplane/MyProduct_Instances.thy
@@ -515,5 +515,4 @@ instance
   done
 end
 
-
 end
